Exersises for Binary Searc Trees

BinSrcTree.v
@@ -62,48 +62,135 @@ Variables Elem : ordType.
 Inductive Tree : Type :=
   | E : Tree
   | T : Tree -> Elem -> Tree -> Tree.
+(* TODO: Invariant of Binary Search Trees *)
+Definition empty : Tree := E.
 
-  Definition empty : Tree := E.
-
-  Fixpoint member (x : Elem) (Tr : Tree) : bool :=
-    if Tr is (T a y b) then 
-        if 
-          lt x y then member x a
-        else 
-          if lt y x 
-            then member x b
-          else true
-    else false.
-
-  Fixpoint member_candidate' (x : Elem) (Tr : Tree) (candidate : option Elem) : bool :=
-  if Tr is T a y b then
-    if lt x y then 
-      member_candidate' x a candidate
-    else
-      member_candidate' x b (Some y)
-  else
-    if candidate is Some cand then
-      if eq x cand then
-        true
-      else false
-    else false.
-
-  Definition member_candidate (x : Elem) (Tr : Tree) := member_candidate' x Tr None.
-
-  Theorem member_eqviv : forall x Tr, member x Tr = member_candidate x Tr.
-  Proof.
-  Admitted.
-  
-
-  Fixpoint insert (x : Elem) (Tr : Tree) : Tree :=
+Fixpoint member (x : Elem) (Tr : Tree) : bool :=
   if Tr is (T a y b) then 
-    if lt x y then
-      T (insert x a) y b
-    else 
-      if lt y x then
-        T a y (insert x b)
-      else T a y b
-  else T E x E.
+      if 
+        lt x y then member x a
+      else 
+        if lt y x 
+          then member x b
+        else true
+  else false.
+
+(* In the worst case, member performs ap-
+proximately 2d comparisons, where d is the depth of the tree. memder_candidate
+takes no more than d + 1 comparisons by keeping track of a candidate ele-
+ment that might be equal to the query element (the last element for which
+< returned false) and checking for equality only when hits the bottom of the tree. *)
+Fixpoint member_candidate' (x : Elem) (Tr : Tree) (candidate : option Elem) : bool :=
+if Tr is T a y b then
+  if lt x y then 
+    member_candidate' x a candidate
+  else
+    member_candidate' x b (Some y)
+else
+  if candidate is Some cand then
+    if eq x cand then
+      true
+    else false
+  else false.
+
+Definition member_candidate (x : Elem) (Tr : Tree) := member_candidate' x Tr None.
+
+Theorem member_eqviv : forall x Tr, member x Tr = member_candidate x Tr.
+Proof.
+Admitted.
+  
+(* Inserting an existing element into a binary search tree copies the
+entire search path even though the copied nodes are indistinguishable from the
+originals. insert_except uses option to avoid this copying. Established only
+one handler per insertion rather than one handler per iteration. *)
+Fixpoint insert (x : Elem) (Tr : Tree) : Tree :=
+if Tr is T a y b then 
+  if lt x y then
+    T (insert x a) y b
+  else 
+    if lt y x then
+      T a y (insert x b)
+    else T a y b
+else T E x E.
+
+Fixpoint insert_except' (x : Elem) (Tr : Tree) : option Tree :=
+if Tr is T a y b then 
+  if lt x y then
+    if insert_except' x a is Some t then
+      Some (T t y b)
+    else None
+  else
+    if lt y x then
+      if insert_except' x b is Some t then
+        Some (T a y t)
+      else None
+    else None
+else Some (T E x E).
+
+Definition insert_except (x : Elem) (Tr : Tree) : Tree :=
+if insert_except' x Tr is Some t then t else Tr.
+
+(* Combined the ideas of the previous two exercises to obtain a ver-
+sion of insert that performs no unnecessary copying and uses no more than
+d + 1 comparisons. *)
+Fixpoint insert_except_candidate' (x : Elem) (Tr : Tree) (candidate : option Elem) : option Tree :=
+if Tr is  T a y b then
+  if lt x y then
+    if insert_except_candidate' x a candidate is Some t then
+      Some (T t y b)
+    else None
+  else insert_except_candidate' x b (Some y)
+else
+  if candidate is Some cand then
+    None
+  else Some (T E x E).
+
+Definition insert_except_candidate (x : Elem) (Tr : Tree) : Tree :=
+  if insert_except_candidate' x Tr None is Some t then t else Tr.
+
+Theorem insert_eqviv1 : forall x y Tr, 
+  member x (insert y Tr) = member x (insert_except y Tr).
+Proof.
+Admitted.
+
+Theorem insert_eqviv2 : forall x y Tr, 
+  member x (insert y Tr) = member x (insert_except_candidate y Tr).
+Proof.
+Admitted.
+    
+(*  Sharing can also be useful within a single object, not just be-
+tween objects. For example, if the two subtrees of a given node are identical,
+then they can be represented by the same tree. *)
+
+(*Using this idea, function complete of type Elem x int -> Tree
+where complete (x, d) creates a complete binary tree of depth d with x
+stored in every node.*)
+
+Fixpoint complete (x : Elem) (d : nat) : Tree :=
+  if d is d'.+1 then let t := complete x d' in T t x t
+  else E.
+
+(* ctreate extends comlete to create balanced trees of arbitrary size. These trees
+  will not always be complete binary trees, but should be as balanced as
+  possible: for any given node, the two subtrees should differ in size by at
+  most one. This function runs in O(log n) time (considering thet division and 
+  submision takes O(1)). *)
+Fixpoint div2 (n : nat) :=
+  match n with
+  | S (S n) => div2 n
+  | _       => O
+  end.
+
+Program Fixpoint create (x : Elem) (m : nat) {mesure m} : Tree :=
+  if m is m'.+1 then
+    let n := div2 m' in
+    if eqn n (m' - n) then
+      let t := complete x n in T t x t
+    else T (create x n) x (create x (n.+1))
+  else E.
+Next Obligation.
+  exact nat.
+Qed.
 
 End TreeDef.
 
